Remove /proverOpt:O:smt.case_split=1 flag for LinearDList.i.dfy

lib/DataStructures/LinearDList.i.dfy
@@ -3,6 +3,14 @@ include "../Base/Option.s.dfy"
 include "../Lang/LinearSequence.s.dfy"
 include "../Lang/LinearSequence.i.dfy"
 
+/*
+In a test of 100 random seeds:
+- this file, as is, succeeded 82 times
+- with the (commented-out) PointerInRange edits, it succeeded 84 times
+- with /proverOpt:O:smt.case_split=1, which had helped with earlier Dafny/Boogie/Z3, only 57 times
+The problem seems to be with Z3 not instantiating quantifiers in some cases.
+*/
+
 module DList {
   import opened NativeTypes
   import opened Options
@@ -30,22 +38,22 @@ module DList {
   ghost const unused:int := -2
   ghost const sentinel:int := -1
 
-  predicate PointerInRange<A>(nodes:seq<Node<A>>, f:seq<int>, i:nat)
-  requires i < |f|
-  {
-    0 < f[i] < |nodes|
-  }
-
-  lemma RevealPointerInRange<A>(nodes:seq<Node<A>>, f:seq<int>)
-  requires forall i :: 0 <= i < |f| ==> PointerInRange(nodes, f, i)
-  ensures forall i :: 0 <= i < |f| ==> 0 < f[i] < |nodes|
-  {
-    forall i | 0 <= i < |f|
-    ensures 0 < f[i] < |nodes|
-    {
-      assert PointerInRange(nodes, f, i);
-    }
-  }
+//  predicate PointerInRange<A>(nodes:seq<Node<A>>, f:seq<int>, i:nat)
+//  requires i < |f|
+//  {
+//    0 < f[i] < |nodes|
+//  }
+//
+//  lemma RevealPointerInRange<A>(nodes:seq<Node<A>>, f:seq<int>)
+//  requires forall i :: 0 <= i < |f| ==> PointerInRange(nodes, f, i)
+//  ensures forall i :: 0 <= i < |f| ==> 0 < f[i] < |nodes|
+//  {
+//    forall i | 0 <= i < |f|
+//    ensures 0 < f[i] < |nodes|
+//    {
+//      assert PointerInRange(nodes, f, i);
+//    }
+//  }
 
   predicate Invs<A>(nodes:seq<Node<A>>, freeStack:uint64, s:seq<A>, f:seq<int>, g:seq<int>)
   {
@@ -54,9 +62,9 @@ module DList {
     && |nodes| > 0
     && g[0] == sentinel
     && 0 <= freeStack as int < |nodes|
-    && (forall i :: 0 <= i < |f| ==> PointerInRange(nodes, f, i))
+    && (forall i {:trigger f[i]} :: 0 <= i < |f| ==> 0 < f[i] < |nodes|) // (forall i :: 0 <= i < |f| ==> PointerInRange(nodes, f, i))
     && (forall i {:trigger g[f[i]]} :: 0 <= i < |f| ==> (
-      assert PointerInRange(nodes, f, i);
+//      assert PointerInRange(nodes, f, i);
       g[f[i]] == i
     ))
     && (forall p :: 0 <= p < |g| ==>
@@ -214,14 +222,14 @@ module DList {
       inout self.freeStack := len' - 1;
       inout ghost self.g := seq(|self.nodes|, i requires 0 <= i < |self.nodes| => if i < |self.g| then self.g[i] else unused);
 
-      forall i | 0 <= i < |self.f|
-      ensures PointerInRange(self.nodes, self.f, i)
-      {
-        assert PointerInRange(old_self.nodes, old_self.f, i); // observe
-      }
-      
-      RevealPointerInRange(old_self.nodes, old_self.f);
-      RevealPointerInRange(self.nodes, self.f);
+//      forall i | 0 <= i < |self.f|
+//      ensures PointerInRange(self.nodes, self.f, i)
+//      {
+//        assert PointerInRange(old_self.nodes, old_self.f, i); // observe
+//      }
+//      
+//      RevealPointerInRange(old_self.nodes, old_self.f);
+//      RevealPointerInRange(self.nodes, self.f);
     }
 
     linear inout method Remove(p:uint64)
@@ -252,16 +260,16 @@ module DList {
       inout ghost self.f := f';
       inout ghost self.g := g';
 
-      forall i | 0 <= i < |self.f|
-      ensures PointerInRange(self.nodes, self.f, i)
-      ensures 0 < self.f[i] < |self.nodes|
-      {
-        if i < index {
-          assert PointerInRange(old_self.nodes, old_self.f, i); // observe
-        } else {
-          assert PointerInRange(old_self.nodes, old_self.f, i + 1); // observe
-        }
-      }
+//      forall i | 0 <= i < |self.f|
+//      ensures PointerInRange(self.nodes, self.f, i)
+//      ensures 0 < self.f[i] < |self.nodes|
+//      {
+//        if i < index {
+//          assert PointerInRange(old_self.nodes, old_self.f, i); // observe
+//        } else {
+//          assert PointerInRange(old_self.nodes, old_self.f, i + 1); // observe
+//        }
+//      }
     }
 
     linear inout method InsertAfter(p:uint64, a:A) returns (p':uint64)
@@ -283,11 +291,11 @@ module DList {
 
       ghost var selfBefore := self;
 
-      forall i | 0 <= i < |selfBefore.f|
-      ensures PointerInRange(selfBefore.nodes, selfBefore.f, i)
-      {
-        assert PointerInRange(self.nodes, self.f, i); // observe
-      }
+//      forall i | 0 <= i < |selfBefore.f|
+//      ensures PointerInRange(selfBefore.nodes, selfBefore.f, i)
+//      {
+//        assert PointerInRange(self.nodes, self.f, i); // observe
+//      }
 
       // linear var DList(nodes, freeStack, s, f, g) := l';
       ghost var index := self.g[p];
@@ -303,21 +311,21 @@ module DList {
       mut_seq_set(inout self.nodes, node.next, node_next.(prev := p'));
       mut_seq_set(inout self.nodes, p', node');
 
-      forall i | 0 <= i < |self.f|
-      ensures PointerInRange(self.nodes, self.f, i)
-      {
-        if i < index {
-          assert PointerInRange(selfBefore.nodes, selfBefore.f, i); // observe
-        } else if i == index {
-        } else if (i as int - 1 >= 0) {
-          assert PointerInRange(selfBefore.nodes, selfBefore.f, i - 1); // observe
-        }
-      }
-
-      assert self.Inv() by {
-        RevealPointerInRange(selfBefore.nodes, selfBefore.f);
-        RevealPointerInRange(self.nodes, self.f);
-      }
+//      forall i | 0 <= i < |self.f|
+//      ensures PointerInRange(self.nodes, self.f, i)
+//      {
+//        if i < index {
+//          assert PointerInRange(selfBefore.nodes, selfBefore.f, i); // observe
+//        } else if i == index {
+//        } else if (i as int - 1 >= 0) {
+//          assert PointerInRange(selfBefore.nodes, selfBefore.f, i - 1); // observe
+//        }
+//      }
+//
+//      assert self.Inv() by {
+//        RevealPointerInRange(selfBefore.nodes, selfBefore.f);
+//        RevealPointerInRange(self.nodes, self.f);
+//      }
     }
 
     linear inout method InsertBefore(p:uint64, a:A) returns(p':uint64)
@@ -340,11 +348,11 @@ module DList {
 
       ghost var selfBefore := self;
 
-      forall i | 0 <= i < |selfBefore.f|
-      ensures PointerInRange(selfBefore.nodes, selfBefore.f, i)
-      {
-        assert PointerInRange(self.nodes, self.f, i); // observe
-      }
+//      forall i | 0 <= i < |selfBefore.f|
+//      ensures PointerInRange(selfBefore.nodes, selfBefore.f, i)
+//      {
+//        assert PointerInRange(self.nodes, self.f, i); // observe
+//      }
 
       //linear var DList(nodes, freeStack, s, f, g) := l';
       ghost var index' := self.IndexHi(p);
@@ -359,28 +367,28 @@ module DList {
       mut_seq_set(inout self.nodes, node.prev, node_prev.(next := p'));
       mut_seq_set(inout self.nodes, p', node');
 
-      forall i | 0 <= i < |self.f|
-      ensures PointerInRange(self.nodes, self.f, i)
-      {
-        if i < index' {
-          assert PointerInRange(selfBefore.nodes, selfBefore.f, i); // observe
-        } else if i == index' {
-        } else {
-          assert PointerInRange(selfBefore.nodes, selfBefore.f, i - 1); // observe
-        }
-      }
-
-      assert self.Inv() by {
-        forall i | 0 <= i < |self.f|
-        ensures (
-          assert PointerInRange(self.nodes, self.f, i);
-          self.g[self.f[i]] == i
-        )
-        {
-          if i == index' {
-          }
-        }
-      }
+//      forall i | 0 <= i < |self.f|
+//      ensures PointerInRange(self.nodes, self.f, i)
+//      {
+//        if i < index' {
+//          assert PointerInRange(selfBefore.nodes, selfBefore.f, i); // observe
+//        } else if i == index' {
+//        } else {
+//          assert PointerInRange(selfBefore.nodes, selfBefore.f, i - 1); // observe
+//        }
+//      }
+//
+//      assert self.Inv() by {
+//        forall i | 0 <= i < |self.f|
+//        ensures (
+//          assert PointerInRange(self.nodes, self.f, i);
+//          self.g[self.f[i]] == i
+//        )
+//        {
+//          if i == index' {
+//          }
+//        }
+//      }
     }
 
     shared method Clone() returns(linear l':DList<A>)
